# Differentiation

## Basic Derivative Practice

1. $W(r) = r^3 + 5r - 12$
1. $f(x) = x^2 - 3\ln x$
1. $P(t) = 4t^2 + 7\sin t$
1. $f(x) = 1/x^2 + 5\sqrt{x} - 7$
1. $s(x) = 2e^{x} + x^2$
1. $h(\theta) = 1/\sqrt[3]{\theta}$
1. $b(t) = t^2 + 5\cos t$


## More Basic Derivative Practice

1. $g(x) = -\frac{1}{2}\left(x^5 +2x -9 \right)$
1. $s(t) = 6t^{-2} + 3t^3 - 4t^{1/2}$
1. $q(x) = 3x - 2\cdot 4^x$
1. $y(x) = \sqrt{x}(x+1)$
1. $P(t) = 3000(1.02)^t$
1. $f(x) = 2^x + x^2 + 1$
1. $d(r) = Ae^{r}  - Br^2 + C$
1. $s(t) = t^2 + 2\ln t$
1. $g(x) = 2x - \frac{1}{\sqrt[3]{x}} + 3^x - e$
1. $y(g) = 5\sin g - 5g + 4$


## Product Rule and Quotient Rule Practice


1. $s(t)=(t^2+4)(5t-1)$
1. $y(x)=x^2\ln x$
1. $g(x)= \frac{25x^2}{e^x}$
1. $h(t)=\frac{t+4}{t-4}$
1. $y(x)=x^2\cos x$

<!--

1. $s'(t) = 2t(5t-1) + (t^2+4)5$
1. $y'(x) = 2x\ln x + x^2 \cdot 1/x$
1. $f'(x) = 50xe^{-x} - 25x^2e^{-x}$
1. $h'(t) = \frac{(t-4) - (t+4)}{(t-4)^2}$
1. $y'(x) = 2x\cos x - x^2\sin x$

-->








## Chain Rule Practice

1. $g(z)=(z^2+5)^3$
1. $g(m) = 200 e^{0.12m}$
1. $h(x) = e^{5x^2+1}$
1. $g(x) = \sqrt{1+x^3}$
1. $f(t) = \cos(2t^3+5t^2)$
1. $k(x) = \ln(4x^2)$

<!--
Solutions

1. $g'(z) = 3(z^2+5)^2\cdot 2z$
1. $g'(m) = 200 \cdot 0.12 \cdot e^{0.12m}$
1. $h'(x) = e^{5x^2+1}\cdot (10x)$
1. $g'(x) = \frac{1}{2}(1+x^3)^{-1/2}\cdot(3x^2)$
1. $f'(t) = -\sin(2t^3+5t^2)\cdot(6t^2+10t)$
1. $k'(x) = \frac{1}{4x^2}\cdot 8x$
-->

## More Chain Rule Practice

1. $f(x)=\sin(2x)$
1. $P(t)=e^{2t}$
1. $y(x)=x e^{3x}$
1. $f(z)=\ln(z^2+1)$
1. $R(t)=(\sin t)^5$
1. $f(t)=\sin \sqrt{e^{t}+1}$
1. $g(y)=e^{2e^{y^3}}$




<!--
1. $f'(x) = 2\cos(2x)$
1. $P'(t) = 2e^{2t}$
1. $y'(x) = e^{3x} + 3xe^{3x}$
1. $f'(z) = \frac{2z}{z^2+1}$
1. $R'(t) = 5 (\sin t)^4 \cdot \cos t$
1. $f'(t) = \cos \sqrt{e^{t}+1} \cdot \frac{1}{2}\left(e^{t}+1\right)^{-1/2}\cdot e^{t}$
1. $g'(y) = e^{2e^{y^3}} \cdot 2e^{y^3}\cdot 3y^2$

-->








<!--

## Basic

1. $W'(r) = 3r^2 + 5$
1. $f'(x) = 2x - 3/x$
1. $P'(t) = 8t + 7\cos t$
1. $f'(x) = -2x^{-3} + \frac{5}{2}x^{-1/2}$
1. $s'(x) = 2e^{x} + 2x$
1. $h'(\theta) = -\frac{1}{3}\theta^{-4/3}$
1. $b'(t) = 2t - 5\sin t$


# More 

1. $g'(x) = -\frac{1}{2}(5x^4 + 2)$
1. $s'(t) = -12 t^{-3} + 9t^2 -2t^{-1/2}$
1. $q'(x) = 3 - 2\cdot \ln 4 \cdot 4^x$
1. $y'(x) = \frac{3}{2}x^{1/2} + \frac{1}{2}x^{-1/2}$
1. $P'(t) = 3000\cdot \ln 1.02 \cdot (1.02)^t$
1. $f'(x) = \ln 2 \cdot 2^x + 2x$
1. $d'(r) = Ae^{r} - 2Br$
1. $s'(t) = 2t + 2/t$
1. $g'(x) = 2 + \frac{1}{3}x^{-4/3} + \ln 3 \cdot 3^x $
1. $y'(g) = 5\cos g - 5$

-->